Revert "update"
This reverts commit eaab822e2a69900d7772cc17d9f66c7ff1e06409.

Abstract_Value_Flow_Analysis.thy
@@ -207,91 +207,13 @@ inductive flow_over_stack :: "abstract_env \<times> abstract_env \<Rightarrow> a
 
 
 inductive flow_over_state :: "abstract_env \<times> abstract_env \<Rightarrow> state \<Rightarrow> bool" (infix "\<TTurnstile>" 55) where
-  Result: "
+  Any: "
     \<lbrakk>
-      (\<V>, \<C>) \<parallel>\<approx> \<rho>;
-      (\<V>, \<C>) \<Turnstile> \<V> x \<Rrightarrow> \<kappa>
-    \<rbrakk> \<Longrightarrow>
-    (\<V>, \<C>) \<TTurnstile> <<RESULT x, \<rho>, \<kappa>>>
-  " |
-  Let_Unit: "
-    \<lbrakk>
-      (\<V>, \<C>) \<Turnstile> (LET x = \<lparr>\<rparr> in e); 
+      (\<V>, \<C>) \<Turnstile> e; 
       (\<V>, \<C>) \<parallel>\<approx> \<rho>; 
       (\<V>, \<C>) \<Turnstile> \<V> (\<lfloor>e\<rfloor>) \<Rrightarrow> \<kappa>
     \<rbrakk> \<Longrightarrow>
-    (\<V>, \<C>) \<TTurnstile> <<LET x = \<lparr>\<rparr> in e, \<rho>, \<kappa>>>
-  " |
-  Let_Chan: "
-    \<lbrakk>
-      (\<V>, \<C>) \<Turnstile> (LET x = CHAN \<lparr>\<rparr> in e); 
-      (\<V>, \<C>) \<parallel>\<approx> \<rho>; 
-      (\<V>, \<C>) \<Turnstile> \<V> (\<lfloor>e\<rfloor>) \<Rrightarrow> \<kappa>
-    \<rbrakk> \<Longrightarrow>
-    (\<V>, \<C>) \<TTurnstile> <<LET x = CHAN \<lparr>\<rparr> in e, \<rho>, \<kappa>>>
-  " |
-  Abs: "
-    \<lbrakk>
-      (\<V>, \<C>) \<Turnstile> (LET x = FN f x\<^sub>l . e\<^sub>l in e); 
-      (\<V>, \<C>) \<parallel>\<approx> \<rho>; 
-      (\<V>, \<C>) \<Turnstile> \<V> (\<lfloor>e\<rfloor>) \<Rrightarrow> \<kappa>
-    \<rbrakk> \<Longrightarrow>
-    (\<V>, \<C>) \<TTurnstile> <<LET x = FN f x\<^sub>l . e\<^sub>l in e, \<rho>, \<kappa>>>
-  " |
-  Pair: "
-    \<lbrakk>
-      (\<V>, \<C>) \<Turnstile> (LET x = \<lparr>x\<^sub>1, x\<^sub>2\<rparr> in e); 
-      (\<V>, \<C>) \<parallel>\<approx> \<rho>; 
-      (\<V>, \<C>) \<Turnstile> \<V> (\<lfloor>e\<rfloor>) \<Rrightarrow> \<kappa>
-    \<rbrakk>  \<Longrightarrow>
-    (\<V>, \<C>) \<TTurnstile> <<LET x = \<lparr>x\<^sub>1, x\<^sub>2\<rparr> in e, \<rho>, \<kappa>>>
-  " |
-  Left: "
-    \<lbrakk>
-      (\<V>, \<C>) \<Turnstile> (LET x = LEFT x\<^sub>p in e); 
-      (\<V>, \<C>) \<parallel>\<approx> \<rho>; 
-      (\<V>, \<C>) \<Turnstile> \<V> (\<lfloor>e\<rfloor>) \<Rrightarrow> \<kappa>
-    \<rbrakk> \<Longrightarrow>
-    (\<V>, \<C>) \<TTurnstile> <<LET x = LEFT x\<^sub>p in e, \<rho>, \<kappa>>>
-  " |
-  Right: "
-    \<lbrakk>
-      (\<V>, \<C>) \<Turnstile> (LET x = RIGHT x\<^sub>p in e); 
-      (\<V>, \<C>) \<parallel>\<approx> \<rho>; 
-      (\<V>, \<C>) \<Turnstile> \<V> (\<lfloor>e\<rfloor>) \<Rrightarrow> \<kappa>
-    \<rbrakk> \<Longrightarrow>
-    (\<V>, \<C>) \<TTurnstile> <<LET x = RIGHT x\<^sub>p in e, \<rho>, \<kappa>>>
-  " |
-  Send_Evt: "
-    \<lbrakk>
-      (\<V>, \<C>) \<Turnstile> (LET x = SEND EVT x\<^sub>c x\<^sub>m in e); 
-      (\<V>, \<C>) \<parallel>\<approx> \<rho>; 
-      (\<V>, \<C>) \<Turnstile> \<V> (\<lfloor>e\<rfloor>) \<Rrightarrow> \<kappa>
-    \<rbrakk> \<Longrightarrow>
-    (\<V>, \<C>) \<TTurnstile> <<LET x = SEND EVT x\<^sub>c x\<^sub>m in e, \<rho>, \<kappa>>>
-  " |
-  Recv_Evt: "
-    \<lbrakk>
-      (\<V>, \<C>) \<Turnstile> (LET x = RECV EVT x\<^sub>c in e); 
-      (\<V>, \<C>) \<parallel>\<approx> \<rho>; 
-      (\<V>, \<C>) \<Turnstile> \<V> (\<lfloor>e\<rfloor>) \<Rrightarrow> \<kappa>
-    \<rbrakk> \<Longrightarrow>
-    (\<V>, \<C>) \<TTurnstile> <<LET x = RECV EVT x\<^sub>c in e, \<rho>, \<kappa>>>
-  " |
-  Always_Evt: "
-    \<lbrakk>
-      (\<V>, \<C>) \<Turnstile> (LET x = ALWAYS EVT x\<^sub>c in e); 
-      (\<V>, \<C>) \<parallel>\<approx> \<rho>; 
-      (\<V>, \<C>) \<Turnstile> \<V> (\<lfloor>e\<rfloor>) \<Rrightarrow> \<kappa>
-    \<rbrakk> \<Longrightarrow>
-    (\<V>, \<C>) \<TTurnstile> <<LET x = ALWAYS EVT x\<^sub>c in e, \<rho>, \<kappa>>>
-  " |
-  Let_Spawn: "
-    \<lbrakk>
-      (\<V>, \<C>) \<TTurnstile> <<e, \<rho>, \<kappa>>>;
-      (\<V>, \<C>) \<TTurnstile> <<e\<^sub>c, \<rho>, \<kappa>>>
-    \<rbrakk> \<Longrightarrow>
-    (\<V>, \<C>) \<TTurnstile> <<LET x = SPAWN e\<^sub>c in e, \<rho>, \<kappa>>>
+    (\<V>, \<C>) \<TTurnstile> <<e, \<rho>, \<kappa>>>
   "
 
 inductive flow_over_pool :: "abstract_env \<times> abstract_env \<Rightarrow> state_pool \<Rightarrow> bool" (infix "\<parallel>\<lless>" 55) where
@@ -301,60 +223,429 @@ inductive flow_over_pool :: "abstract_env \<times> abstract_env \<Rightarrow> st
     (\<V>, \<C>) \<parallel>\<lless> \<E>
   "
 
-lemma flow_over_state_1: "
-  (\<V>, \<C>) \<TTurnstile> <<RESULT x, \<rho>, \<langle>x\<^sub>\<kappa>,e\<^sub>\<kappa>,\<rho>\<^sub>\<kappa>\<rangle> # \<kappa>'>> \<Longrightarrow>
-  \<rho> x = Some \<omega> \<Longrightarrow>
-  (\<V>, \<C>) \<TTurnstile> <<e\<^sub>\<kappa>,\<rho>\<^sub>\<kappa>(x\<^sub>\<kappa> \<mapsto> \<omega>),\<kappa>'>>
+lemma flow_state_to_flow_exp: "
+  (\<V>, \<C>) \<TTurnstile> <<RESULT x,\<rho>,\<langle>x\<^sub>\<kappa>,e\<^sub>\<kappa>,\<rho>\<^sub>\<kappa>\<rangle> # \<kappa>>> \<Longrightarrow> \<rho> x = Some \<omega> \<Longrightarrow> (\<V>, \<C>) \<Turnstile> e\<^sub>\<kappa>
 "
-sorry
+ apply (erule flow_over_state.cases, auto)
+ apply (erule flow_over_stack.cases, auto)
+done
+
+lemma flow_over_state_to_env: "
+  (\<V>, \<C>) \<TTurnstile> <<RESULT x,\<rho>,\<langle>x\<^sub>\<kappa>,e\<^sub>\<kappa>,\<rho>\<^sub>\<kappa>\<rangle> # \<kappa>>> \<Longrightarrow> \<rho> x = Some \<omega> \<Longrightarrow> 
+  (\<V>, \<C>) \<parallel>\<approx> \<rho>\<^sub>\<kappa>(x\<^sub>\<kappa> \<mapsto> \<omega>)
+"
+ apply (rule flow_over_value_flow_over_env.Any, auto)
+    apply (erule flow_over_state.cases, auto)
+    apply (erule flow_over_env.cases, auto)
+    apply (erule flow_over_stack.cases, auto)
+   apply (erule flow_over_state.cases, auto)
+   apply (erule flow_over_env.cases, auto)
+  apply (rename_tac x' \<omega>')
+  apply (erule flow_over_state.cases, auto)
+  apply (erule flow_over_env.cases, auto)
+  apply (drule spec)+
+  apply (erule impE, auto)
+  apply (erule flow_over_stack.cases, auto)+
+  apply (erule flow_over_env.cases, auto)+
+  apply (rename_tac x' \<omega>')
+ apply (erule flow_over_state.cases, auto)
+ apply (erule flow_over_env.cases, auto)
+ apply (drule spec)+
+ apply (erule impE, auto)
+ apply (erule flow_over_stack.cases, auto)+
+ apply (erule flow_over_env.cases, auto)+
+done
+
+lemma flow_over_state_to_stack: "
+  (\<V>, \<C>) \<TTurnstile> <<RESULT x,\<rho>,\<langle>x\<^sub>\<kappa>,e\<^sub>\<kappa>,\<rho>\<^sub>\<kappa>\<rangle> # \<kappa>>> \<Longrightarrow> \<rho> x = Some \<omega> \<Longrightarrow> (\<V>, \<C>) \<Turnstile> \<V> (\<lfloor>e\<^sub>\<kappa>\<rfloor>) \<Rrightarrow> \<kappa>
+"
+ apply (erule flow_over_state.cases, auto)
+ apply (erule flow_over_env.cases, auto)
+ apply (drule spec)+
+ apply (erule impE, auto)
+ apply (erule flow_over_stack.cases, auto)+
+done
+
+lemma flow_over_state_1: "
+  (\<V>, \<C>) \<TTurnstile> <<RESULT x,\<rho>,\<langle>x\<^sub>\<kappa>,e\<^sub>\<kappa>,\<rho>\<^sub>\<kappa>\<rangle> # \<kappa>>> \<Longrightarrow> \<rho> x = Some \<omega> \<Longrightarrow> (\<V>, \<C>) \<TTurnstile> <<e\<^sub>\<kappa>,\<rho>\<^sub>\<kappa>(x\<^sub>\<kappa> \<mapsto> \<omega>),\<kappa>>>
+"
+ apply (rule flow_over_state.Any)
+    apply (erule flow_state_to_flow_exp, auto)
+   apply (erule flow_over_state_to_env, auto)
+  apply (erule flow_over_state_to_stack, auto)
+done
+
+lemma flow_state_to_flow_exp_2: "
+  (\<V>, \<C>) \<TTurnstile> <<LET x = \<lparr>\<rparr> in e,\<rho>,\<kappa>>> \<Longrightarrow> (\<V>, \<C>) \<Turnstile> e
+"
+ apply (erule flow_over_state.cases, auto)
+ apply (erule flow.cases, auto)
+done
+
+lemma flow_over_state_to_env_2: "
+  (\<V>, \<C>) \<TTurnstile> <<LET x = \<lparr>\<rparr> in e,\<rho>,\<kappa>>> \<Longrightarrow> (\<V>, \<C>) \<parallel>\<approx> \<rho>(x \<mapsto> \<lbrace>\<rbrace>)
+"
+ apply (rule flow_over_value_flow_over_env.Any, auto)
+    apply (erule flow_over_state.cases, auto)
+    apply (erule flow.cases, auto)
+   apply (rule flow_over_value_flow_over_env.Unit)
+  apply (rename_tac x' \<omega>')
+  apply (erule flow_over_state.cases, auto)
+  apply (erule flow_over_env.cases, auto)
+ apply (erule flow_over_state.cases, auto)
+ apply (erule flow_over_env.cases, auto)
+done
+
+lemma flow_over_state_to_stack_2: "
+  (\<V>, \<C>) \<TTurnstile> <<LET x = \<lparr>\<rparr> in e,\<rho>,\<kappa>>> \<Longrightarrow> (\<V>, \<C>) \<Turnstile> \<V> (\<lfloor>e\<rfloor>) \<Rrightarrow> \<kappa>
+"
+ apply (erule flow_over_state.cases, auto)
+done
 
 lemma flow_over_state_2: "
   (\<V>, \<C>) \<TTurnstile> <<LET x = \<lparr>\<rparr> in e,\<rho>,\<kappa>>> \<Longrightarrow> (\<V>, \<C>) \<TTurnstile> <<e,\<rho>(x \<mapsto> \<lbrace>\<rbrace>),\<kappa>>>
 "
-sorry
+ apply (rule flow_over_state.Any)
+    apply (erule flow_state_to_flow_exp_2)
+   apply (erule flow_over_state_to_env_2)
+  apply (erule flow_over_state_to_stack_2)
+done
+
+lemma flow_over_state_to_exp_3: "
+  (\<V>, \<C>) \<TTurnstile> <<LET x = Prim p in e,\<rho>,\<kappa>>> \<Longrightarrow> (\<V>, \<C>) \<Turnstile> e
+"
+ apply (erule flow_over_state.cases, auto)  
+ apply (erule flow.cases, auto)
+done
+
+lemma flow_over_state_to_env_3: "
+  (\<V>, \<C>) \<TTurnstile> <<LET x = Prim p in e,\<rho>,\<kappa>>> \<Longrightarrow> (\<V>, \<C>) \<parallel>\<approx> \<rho>(x \<mapsto> \<lbrace>p, \<rho>\<rbrace>)
+"
+ apply (rule flow_over_value_flow_over_env.Any, auto)
+    apply (erule flow_over_state.cases, auto)
+    apply (erule flow.cases, auto)
+   apply (erule flow_over_state.cases, auto)
+   apply ((erule flow.cases, auto); rule, auto)
+  apply (rename_tac x' \<omega>')
+  apply (erule flow_over_state.cases, auto)
+  apply (erule flow_over_env.cases, auto)
+ apply (erule flow_over_state.cases, auto)
+ apply (erule flow_over_env.cases, auto)
+done
+
+lemma flow_over_state_to_stack_3: "
+  (\<V>, \<C>) \<TTurnstile> <<LET x = Prim p in e,\<rho>,\<kappa>>> \<Longrightarrow> (\<V>, \<C>) \<Turnstile> \<V> (\<lfloor>e\<rfloor>) \<Rrightarrow> \<kappa>
+"
+ apply (erule flow_over_state.cases, auto)
+done
 
 lemma flow_over_state_3: "
   (\<V>, \<C>) \<TTurnstile> <<LET x = Prim p in e,\<rho>,\<kappa>>> \<Longrightarrow>  (\<V>, \<C>) \<TTurnstile> <<e,\<rho>(x \<mapsto> \<lbrace>p, \<rho>\<rbrace>),\<kappa>>>
 "
-sorry
+ apply (rule flow_over_state.Any)
+    apply (erule flow_over_state_to_exp_3)
+   apply (erule flow_over_state_to_env_3)
+  apply (erule flow_over_state_to_stack_3)
+done
+
+lemma flow_state_to_flow_exp_4: "
+  (\<V>, \<C>) \<TTurnstile> <<LET x = CASE x\<^sub>s LEFT x\<^sub>l |> e\<^sub>l RIGHT x\<^sub>r |> e\<^sub>r in e,\<rho>,\<kappa>>> \<Longrightarrow> 
+  \<rho> x\<^sub>s = Some \<lbrace>prim.Left x\<^sub>l', \<rho>\<^sub>l\<rbrace> \<Longrightarrow> 
+  \<rho>\<^sub>l x\<^sub>l' = Some \<omega>\<^sub>l \<Longrightarrow> (\<V>, \<C>) \<Turnstile> e\<^sub>l
+"
+ apply (erule flow_over_state.cases, auto)
+ apply (erule flow.cases, auto)
+ apply (erule flow_over_env.cases, auto)
+ apply ((drule spec)+, auto)
+done
+
+lemma flow_state_to_flow_env_4: "
+  (\<V>, \<C>) \<TTurnstile> <<LET x = CASE x\<^sub>s LEFT x\<^sub>l |> e\<^sub>l RIGHT x\<^sub>r |> e\<^sub>r in e,\<rho>,\<kappa>>> \<Longrightarrow> 
+  \<rho> x\<^sub>s = Some \<lbrace>prim.Left x\<^sub>l', \<rho>\<^sub>l\<rbrace> \<Longrightarrow> \<rho>\<^sub>l x\<^sub>l' = Some \<omega>\<^sub>l \<Longrightarrow> 
+  (\<V>, \<C>) \<parallel>\<approx> \<rho>(x\<^sub>l \<mapsto> \<omega>\<^sub>l)
+"
+ apply (rule flow_over_value_flow_over_env.Any, auto)
+    apply (erule flow_over_state.cases, auto)
+    apply (erule flow_over_env.cases, auto)
+    apply ((drule spec)+, auto)
+    apply (erule flow_over_value.cases, auto)
+    apply (erule flow_over_env.cases, auto)
+    apply ((drule spec)+, auto)
+    apply (erule flow.cases, auto)
+   apply (erule flow_over_state.cases, auto)
+   apply (erule flow_over_env.cases, auto)
+   apply ((drule spec)+, auto)
+   apply (erule flow_over_value.cases, auto)
+   apply (erule flow_over_env.cases, auto)
+  apply (rename_tac x' \<omega>')
+  apply (erule flow_over_state.cases, auto)
+  apply (erule flow_over_env.cases, auto)
+ apply (rename_tac x' \<omega>')
+ apply (erule flow_over_state.cases, auto)
+ apply (erule flow_over_env.cases, auto)
+done
+
+lemma flow_state_to_flow_stack_4: "
+  (\<V>, \<C>) \<TTurnstile> <<LET x = CASE x\<^sub>s LEFT x\<^sub>l |> e\<^sub>l RIGHT x\<^sub>r |> e\<^sub>r in e,\<rho>,\<kappa>>> \<Longrightarrow>
+  \<rho> x\<^sub>s = Some \<lbrace>prim.Left x\<^sub>l', \<rho>\<^sub>l\<rbrace> \<Longrightarrow> \<rho>\<^sub>l x\<^sub>l' = Some \<omega>\<^sub>l \<Longrightarrow> 
+  (\<V>, \<C>) \<Turnstile> \<V> (\<lfloor>e\<^sub>l\<rfloor>) \<Rrightarrow> \<langle>x,e,\<rho>\<rangle> # \<kappa>
+"
+ apply (rule flow_over_stack.Nonempty)
+    apply (erule flow_over_state.cases, auto, rename_tac \<omega>)
+    apply (erule flow_over_env.cases, auto)
+    apply ((drule spec)+, auto)
+    apply (erule flow.cases, auto)
+   apply (erule flow_over_state.cases, auto)
+   apply (erule flow.cases, auto)
+  apply (erule flow_over_state.cases, auto)
+ apply (erule flow_over_state.cases, auto)
+done
 
 lemma flow_over_state_4: "
   (\<V>, \<C>) \<TTurnstile> <<LET x = CASE x\<^sub>s LEFT x\<^sub>l |> e\<^sub>l RIGHT x\<^sub>r |> e\<^sub>r in e,\<rho>,\<kappa>>> \<Longrightarrow> 
   \<rho> x\<^sub>s = Some \<lbrace>prim.Left x\<^sub>l', \<rho>\<^sub>l\<rbrace> \<Longrightarrow> 
   \<rho>\<^sub>l x\<^sub>l' = Some \<omega>\<^sub>l \<Longrightarrow> (\<V>, \<C>) \<TTurnstile> <<e\<^sub>l,\<rho>(x\<^sub>l \<mapsto> \<omega>\<^sub>l),\<langle>x,e,\<rho>\<rangle> # \<kappa>>>
 "
-sorry
+ apply (rule flow_over_state.Any)
+    apply (erule flow_state_to_flow_exp_4, simp, auto)
+   apply (erule flow_state_to_flow_env_4, simp, auto)
+  apply (erule flow_state_to_flow_stack_4, simp, auto)
+done
 
+lemma flow_state_to_flow_exp_5: "
+  (\<V>, \<C>) \<TTurnstile> <<LET x = CASE x\<^sub>s LEFT x\<^sub>l |> e\<^sub>l RIGHT x\<^sub>r |> e\<^sub>r in e,\<rho>,\<kappa>>> \<Longrightarrow> 
+  \<rho> x\<^sub>s = Some \<lbrace>prim.Right x\<^sub>r', \<rho>\<^sub>r\<rbrace> \<Longrightarrow> 
+  \<rho>\<^sub>r x\<^sub>r' = Some \<omega>\<^sub>r \<Longrightarrow> (\<V>, \<C>) \<Turnstile> e\<^sub>r
+"
+ apply (erule flow_over_state.cases, auto)
+ apply (erule flow.cases, auto)
+ apply (erule flow_over_env.cases, auto)
+ apply ((drule spec)+, auto)
+done
+
+lemma flow_state_to_flow_env_5: "
+  (\<V>, \<C>) \<TTurnstile> <<LET x = CASE x\<^sub>s LEFT x\<^sub>l |> e\<^sub>l RIGHT x\<^sub>r |> e\<^sub>r in e,\<rho>,\<kappa>>> \<Longrightarrow> 
+  \<rho> x\<^sub>s = Some \<lbrace>prim.Right x\<^sub>r', \<rho>\<^sub>r\<rbrace> \<Longrightarrow> \<rho>\<^sub>r x\<^sub>r' = Some \<omega>\<^sub>r \<Longrightarrow> 
+  (\<V>, \<C>) \<parallel>\<approx> \<rho>(x\<^sub>r \<mapsto> \<omega>\<^sub>r)
+"
+ apply (rule flow_over_value_flow_over_env.Any, auto)
+    apply (erule flow_over_state.cases, auto)
+    apply (erule flow_over_env.cases, auto)
+    apply ((drule spec)+, auto)
+    apply (erule flow_over_value.cases, auto)
+    apply (erule flow_over_env.cases, auto)
+    apply ((drule spec)+, auto)
+    apply (erule flow.cases, auto)
+   apply (erule flow_over_state.cases, auto)
+   apply (erule flow_over_env.cases, auto)
+   apply ((drule spec)+, auto)
+   apply (erule flow_over_value.cases, auto)
+   apply (erule flow_over_env.cases, auto)
+  apply (rename_tac x' \<omega>')
+  apply (erule flow_over_state.cases, auto)
+  apply (erule flow_over_env.cases, auto)
+ apply (rename_tac x' \<omega>')
+ apply (erule flow_over_state.cases, auto)
+ apply (erule flow_over_env.cases, auto)
+done
+
+lemma flow_state_to_flow_stack_5: "
+  (\<V>, \<C>) \<TTurnstile> <<LET x = CASE x\<^sub>s LEFT x\<^sub>l |> e\<^sub>l RIGHT x\<^sub>r |> e\<^sub>r in e,\<rho>,\<kappa>>> \<Longrightarrow>
+  \<rho> x\<^sub>s = Some \<lbrace>prim.Right x\<^sub>r', \<rho>\<^sub>r\<rbrace> \<Longrightarrow> \<rho>\<^sub>r x\<^sub>r' = Some \<omega>\<^sub>r \<Longrightarrow> 
+  (\<V>, \<C>) \<Turnstile> \<V> (\<lfloor>e\<^sub>r\<rfloor>) \<Rrightarrow> \<langle>x,e,\<rho>\<rangle> # \<kappa>
+"
+ apply (rule flow_over_stack.Nonempty)
+    apply (erule flow_over_state.cases, auto, rename_tac \<omega>)
+    apply (erule flow_over_env.cases, auto)
+    apply ((drule spec)+, auto)
+    apply (erule flow.cases, auto)
+   apply (erule flow_over_state.cases, auto)
+   apply (erule flow.cases, auto)
+  apply (erule flow_over_state.cases, auto)
+ apply (erule flow_over_state.cases, auto)
+done
 
 lemma flow_over_state_5: "
   (\<V>, \<C>) \<TTurnstile> <<LET x = CASE x\<^sub>s LEFT x\<^sub>l |> e\<^sub>l RIGHT x\<^sub>r |> e\<^sub>r in e,\<rho>,\<kappa>>> \<Longrightarrow> 
   \<rho> x\<^sub>s = Some \<lbrace>prim.Right x\<^sub>r', \<rho>\<^sub>r\<rbrace> \<Longrightarrow> 
   \<rho>\<^sub>r x\<^sub>r' = Some \<omega>\<^sub>r \<Longrightarrow> (\<V>, \<C>) \<TTurnstile> <<e\<^sub>r,\<rho>(x\<^sub>r \<mapsto> \<omega>\<^sub>r),\<langle>x,e,\<rho>\<rangle> # \<kappa>>>
 "
-sorry
+ apply (rule flow_over_state.Any)
+    apply (erule flow_state_to_flow_exp_5, simp, auto)
+   apply (erule flow_state_to_flow_env_5, simp, auto)
+  apply (erule flow_state_to_flow_stack_5, simp, auto)
+done
 
+
+lemma flow_state_to_flow_exp_6: "
+  (\<V>, \<C>) \<TTurnstile> <<LET x = FST x\<^sub>p in e,\<rho>,\<kappa>>> \<Longrightarrow> \<rho> x\<^sub>p = Some \<lbrace>prim.Pair x\<^sub>1 x\<^sub>2, \<rho>\<^sub>p\<rbrace> \<Longrightarrow> 
+  \<rho>\<^sub>p x\<^sub>1 = Some \<omega> \<Longrightarrow> (\<V>, \<C>) \<Turnstile> e
+"
+ apply (erule flow_over_state.cases, auto)
+ apply (erule flow.cases, auto)
+done
+
+lemma flow_state_to_flow_env_6: "
+  (\<V>, \<C>) \<TTurnstile> <<LET x = FST x\<^sub>p in e,\<rho>,\<kappa>>> \<Longrightarrow> \<rho> x\<^sub>p = Some \<lbrace>prim.Pair x\<^sub>1 x\<^sub>2, \<rho>\<^sub>p\<rbrace> \<Longrightarrow> \<rho>\<^sub>p x\<^sub>1 = Some \<omega> \<Longrightarrow> (\<V>, \<C>) \<parallel>\<approx> \<rho>(x \<mapsto> \<omega>)
+"
+ apply (rule flow_over_value_flow_over_env.Any, auto)
+    apply (erule flow_over_state.cases, auto)
+    apply (erule flow_over_env.cases, auto)
+    apply ((drule spec)+, auto)
+    apply (erule flow_over_value.cases, auto)
+    apply (erule flow_over_env.cases, auto)
+    apply ((drule spec)+, auto)
+    apply (erule flow.cases, auto)
+   apply (erule flow_over_state.cases, auto)
+   apply (erule flow_over_env.cases, auto)
+   apply ((drule spec)+, auto)
+   apply (erule flow_over_value.cases, auto)
+   apply (erule flow_over_env.cases, auto)
+  apply (rename_tac x' \<omega>')
+  apply (erule flow_over_state.cases, auto)
+  apply (erule flow_over_env.cases, auto)
+ apply (rename_tac x' \<omega>')
+ apply (erule flow_over_state.cases, auto)
+ apply (erule flow_over_env.cases, auto)
+done
+
+lemma flow_state_to_flow_stack_6: "
+  (\<V>, \<C>) \<TTurnstile> <<LET x = FST x\<^sub>p in e,\<rho>,\<kappa>>> \<Longrightarrow> \<rho> x\<^sub>p = Some \<lbrace>prim.Pair x\<^sub>1 x\<^sub>2, \<rho>\<^sub>p\<rbrace> \<Longrightarrow> \<rho>\<^sub>p x\<^sub>1 = Some \<omega> \<Longrightarrow> (\<V>, \<C>) \<Turnstile> \<V> (\<lfloor>e\<rfloor>) \<Rrightarrow> \<kappa>
+"
+ apply (erule flow_over_state.cases, auto)
+done
 
 lemma flow_over_state_6: "
   (\<V>, \<C>) \<TTurnstile> <<LET x = FST x\<^sub>p in e,\<rho>,\<kappa>>> \<Longrightarrow>
   \<rho> x\<^sub>p = Some \<lbrace>prim.Pair x\<^sub>1 x\<^sub>2, \<rho>\<^sub>p\<rbrace> \<Longrightarrow> \<rho>\<^sub>p x\<^sub>1 = Some \<omega> \<Longrightarrow> 
   (\<V>, \<C>) \<TTurnstile> <<e,\<rho>(x \<mapsto> \<omega>),\<kappa>>>
 "
-sorry
+ apply (rule flow_over_state.Any)
+    apply (erule flow_state_to_flow_exp_6, simp, auto)
+   apply (erule flow_state_to_flow_env_6, simp, auto)
+  apply (erule flow_state_to_flow_stack_6, simp, auto)
+done
 
+lemma flow_state_to_flow_exp_7: "
+  (\<V>, \<C>) \<TTurnstile> <<LET x = SND x\<^sub>p in e,\<rho>,\<kappa>>> \<Longrightarrow> \<rho> x\<^sub>p = Some \<lbrace>prim.Pair x\<^sub>1 x\<^sub>2, \<rho>\<^sub>p\<rbrace> \<Longrightarrow> 
+  \<rho>\<^sub>p x\<^sub>2 = Some \<omega> \<Longrightarrow> (\<V>, \<C>) \<Turnstile> e
+"
+ apply (erule flow_over_state.cases, auto)
+ apply (erule flow.cases, auto)
+done
+
+lemma flow_state_to_flow_env_7: "
+  (\<V>, \<C>) \<TTurnstile> <<LET x = SND x\<^sub>p in e,\<rho>,\<kappa>>> \<Longrightarrow> \<rho> x\<^sub>p = Some \<lbrace>prim.Pair x\<^sub>1 x\<^sub>2, \<rho>\<^sub>p\<rbrace> \<Longrightarrow> \<rho>\<^sub>p x\<^sub>2 = Some \<omega> \<Longrightarrow> (\<V>, \<C>) \<parallel>\<approx> \<rho>(x \<mapsto> \<omega>)
+"
+ apply (rule flow_over_value_flow_over_env.Any, auto)
+    apply (erule flow_over_state.cases, auto)
+    apply (erule flow_over_env.cases, auto)
+    apply ((drule spec)+, auto)
+    apply (erule flow_over_value.cases, auto)
+    apply (erule flow_over_env.cases, auto)
+    apply ((drule spec)+, auto)
+    apply (erule flow.cases, auto)
+   apply (erule flow_over_state.cases, auto)
+   apply (erule flow_over_env.cases, auto)
+   apply ((drule spec)+, auto)
+   apply (erule flow_over_value.cases, auto)
+   apply (erule flow_over_env.cases, auto)
+  apply (rename_tac x' \<omega>')
+  apply (erule flow_over_state.cases, auto)
+  apply (erule flow_over_env.cases, auto)
+ apply (rename_tac x' \<omega>')
+ apply (erule flow_over_state.cases, auto)
+ apply (erule flow_over_env.cases, auto)
+done
+
+lemma flow_state_to_flow_stack_7: "
+  (\<V>, \<C>) \<TTurnstile> <<LET x = SND x\<^sub>p in e,\<rho>,\<kappa>>> \<Longrightarrow> \<rho> x\<^sub>p = Some \<lbrace>prim.Pair x\<^sub>1 x\<^sub>2, \<rho>\<^sub>p\<rbrace> \<Longrightarrow> \<rho>\<^sub>p x\<^sub>2 = Some \<omega> \<Longrightarrow> (\<V>, \<C>) \<Turnstile> \<V> (\<lfloor>e\<rfloor>) \<Rrightarrow> \<kappa>
+"
+ apply (erule flow_over_state.cases, auto)
+done
 
 lemma flow_over_state_7: "
   (\<V>, \<C>) \<TTurnstile> <<LET x = SND x\<^sub>p in e,\<rho>,\<kappa>>> \<Longrightarrow>
   \<rho> x\<^sub>p = Some \<lbrace>prim.Pair x\<^sub>1 x\<^sub>2, \<rho>\<^sub>p\<rbrace> \<Longrightarrow> \<rho>\<^sub>p x\<^sub>2 = Some \<omega> \<Longrightarrow> 
   (\<V>, \<C>) \<TTurnstile> <<e,\<rho>(x \<mapsto> \<omega>),\<kappa>>>
 "
-sorry
+ apply (rule flow_over_state.Any)
+    apply (erule flow_state_to_flow_exp_7, simp, auto)
+   apply (erule flow_state_to_flow_env_7, simp, auto)
+  apply (erule flow_state_to_flow_stack_7, simp, auto)
+done
+
+lemma flow_state_to_flow_exp_8: "
+ (\<V>, \<C>) \<TTurnstile> <<LET x = APP f x\<^sub>a in e,\<rho>,\<kappa>>> \<Longrightarrow> 
+ \<rho> f = Some \<lbrace>Abs f\<^sub>l x\<^sub>l e\<^sub>l, \<rho>\<^sub>l\<rbrace> \<Longrightarrow> \<rho> x\<^sub>a = Some \<omega>\<^sub>a \<Longrightarrow> 
+ (\<V>, \<C>) \<Turnstile> e\<^sub>l
+"
+ apply (erule flow_over_state.cases, auto)
+ apply (erule flow.cases, auto)
+ apply (erule flow_over_env.cases, auto)
+ apply ((drule spec)+, auto)
+ apply (erule flow_over_value.cases, auto)
+done
+
+lemma flow_state_to_flow_env_8: "
+  (\<V>, \<C>) \<TTurnstile> <<LET x = APP f x\<^sub>a in e,\<rho>,\<kappa>>> \<Longrightarrow> 
+  \<rho> f = Some \<lbrace>Abs f\<^sub>l x\<^sub>l e\<^sub>l, \<rho>\<^sub>l\<rbrace> \<Longrightarrow> \<rho> x\<^sub>a = Some \<omega>\<^sub>a \<Longrightarrow> 
+  (\<V>, \<C>) \<parallel>\<approx> \<rho>\<^sub>l(f\<^sub>l \<mapsto> \<lbrace>Abs f\<^sub>l x\<^sub>l e\<^sub>l, \<rho>\<^sub>l\<rbrace>, x\<^sub>l \<mapsto> \<omega>\<^sub>a)
+"
+ apply (rule flow_over_value_flow_over_env.Any, auto)
+        apply (erule flow_over_state.cases, auto)
+        apply (erule flow.cases, auto, (drule spec)+, auto)
+         apply (erule flow_over_env.cases, auto, (drule spec)+, auto)
+        apply (erule flow_over_env.cases, auto)
+       apply (erule flow_over_state.cases, auto)
+       apply (erule flow_over_env.cases, auto)
+      apply (erule flow_over_state.cases, auto)
+      apply (erule flow_over_env.cases, auto, (drule spec)+, auto)
+      apply (erule flow_over_value.cases, auto)
+     apply (erule flow_over_state.cases, auto)
+     apply (erule flow_over_env.cases, auto)
+    apply (erule flow_over_state.cases, auto)
+    apply (erule flow.cases, auto, (drule spec)+, auto)
+     apply (erule flow_over_env.cases, auto, (drule spec)+, auto)
+    apply (erule flow_over_env.cases, auto)
+   apply (erule flow_over_state.cases, auto)
+   apply (erule flow_over_env.cases, auto)
+  apply (rename_tac x' \<omega>)
+  apply (erule flow_over_state.cases, auto)
+  apply (erule flow_over_env.cases, auto, (drule spec)+, auto)
+  apply (erule flow_over_value.cases, auto)
+  apply (erule flow_over_env.cases, auto)
+ apply (erule flow_over_state.cases, auto)
+ apply (erule flow_over_env.cases, auto, (drule spec)+, auto)
+ apply (erule flow_over_value.cases, auto)
+ apply (erule flow_over_env.cases, auto)
+done
+
+lemma flow_state_to_flow_stack_8: "
+  (\<V>, \<C>) \<TTurnstile> <<LET x = APP f x\<^sub>a in e,\<rho>,\<kappa>>> \<Longrightarrow> 
+  \<rho> f = Some \<lbrace>Abs f\<^sub>l x\<^sub>l e\<^sub>l, \<rho>\<^sub>l\<rbrace> \<Longrightarrow> \<rho> x\<^sub>a = Some \<omega>\<^sub>a \<Longrightarrow> 
+  (\<V>, \<C>) \<Turnstile> \<V> (\<lfloor>e\<^sub>l\<rfloor>) \<Rrightarrow> \<langle>x,e,\<rho>\<rangle> # \<kappa>
+"
+ apply (rule flow_over_stack.Nonempty)
+    apply (erule flow_over_state.cases, auto) 
+    apply (erule flow.cases, auto)
+    apply (erule flow_over_env.cases, (drule spec)+, auto)
+   apply (erule flow_over_state.cases, auto) 
+   apply (erule flow.cases, auto)
+  apply (erule flow_over_state.cases, auto) 
+ apply (erule flow_over_state.cases, auto) 
+done
 
 lemma flow_over_state_8: "
   (\<V>, \<C>) \<TTurnstile> <<LET x = APP f x\<^sub>a in e,\<rho>,\<kappa>>> \<Longrightarrow>
   \<rho> f = Some \<lbrace>Abs f\<^sub>l x\<^sub>l e\<^sub>l, \<rho>\<^sub>l\<rbrace> \<Longrightarrow> \<rho> x\<^sub>a = Some \<omega>\<^sub>a \<Longrightarrow> 
   (\<V>, \<C>) \<TTurnstile> <<e\<^sub>l,\<rho>\<^sub>l(f\<^sub>l \<mapsto> \<lbrace>Abs f\<^sub>l x\<^sub>l e\<^sub>l, \<rho>\<^sub>l\<rbrace>, x\<^sub>l \<mapsto> \<omega>\<^sub>a),\<langle>x,e,\<rho>\<rangle> # \<kappa>>>
 "
-sorry
+ apply (rule flow_over_state.Any)
+    apply (erule flow_state_to_flow_exp_8, simp, auto)
+   apply (erule flow_state_to_flow_env_8, simp, auto)
+  apply (erule flow_state_to_flow_stack_8, simp, auto)
+done
 
 theorem flow_over_state_preservation : "
   \<lbrakk>
@@ -393,7 +684,7 @@ theorem flow_preservation : "
   (\<V>, \<C>) \<parallel>\<lless> \<E>'
 "
  apply (erule concur_step.cases, auto)
-    apply (erule flow_seq_step_preservation, auto)
+  apply (erule flow_seq_step_preservation, auto)
 sorry
 
 theorem flow_preservation_star' : "
@@ -433,7 +724,9 @@ theorem flow_over_state_precision : "
   \<Longrightarrow>
   \<parallel>\<rho>\<parallel> \<sqsubseteq> \<V>
 "
-sorry
+ apply (erule flow_over_state.cases, auto)
+ apply (erule flow_over_env_precision)
+done
 
 lemma flow_over_pool_to_state: "
   \<lbrakk>
@@ -462,7 +755,9 @@ theorem flow_over_pool_precision : "
 done
 
 theorem lift_flow_exp_to_state: "(\<V>, \<C>) \<Turnstile> e \<Longrightarrow> (\<V>, \<C>) \<TTurnstile> <<e, empty, []>>"
-sorry
+ apply (rule flow_over_state.Any, auto)
+ apply (rule+, auto, rule)
+done
 
 theorem  lift_flow_state_to_pool: "(\<V>, \<C>) \<TTurnstile> \<sigma> \<Longrightarrow> (\<V>, \<C>) \<parallel>\<lless> [[] \<mapsto> \<sigma>]"
   apply (rule flow_over_pool.Any)
